raw type in nonterminal

LottExamples/LeanEscape.lean
@@ -1,4 +1,5 @@
 import Lott
+import Lott.Elab.Nat
 
 namespace LottExamples.LeanEscape
 
@@ -9,15 +10,35 @@ nonterminal Term, e :=
 nonterminal Ty, τ :=
   | "Top" : top
 
+nonterminal Env, Γ :=
+  | "mk " type(Nat -> Term) : mk
+
 judgement_syntax e " : " τ : HasType
 
 judgement HasType := fun e τ => e = [[unit]] ∧ τ = [[Top]]
 
 def wrappedUnit : Term := [[lean% Term.wrap Term.unit]]
+def trivialEnv : Env := [[mk [[lean% (fun _ => Term.unit)]]]]
 
 example : [[unit : [[lean% Ty.top]]]] := by
   exact And.intro rfl rfl
 
 example : wrappedUnit = Term.wrap Term.unit := rfl
+example : trivialEnv = Env.mk (fun _ => Term.unit) := rfl
+
+nonterminal MyList, ρ :=
+  | "mk " type(List Term) : «mk»
+  | "append(" ρ ", " ρ' ")" : app
+
+judgement_syntax ρ "is of length" n : MyListLength
+judgement MyListLength where
+
+───────────────────────────────── base
+[[lean% .mk .nil]] is of length 0
+
+ρ is of length n
+ρ' is of length n
+───────────────────────────────── app
+append(ρ, ρ') is of length n
 
 end LottExamples.LeanEscape
